Add optimizable bulk operations to Actions, native and external SetReaders (#6274)

Source/DafnyCore/Backends/GoLang/GoCodeGenerator.cs
@@ -48,7 +48,8 @@ namespace Microsoft.Dafny.Compilers {
       Feature.ExternalConstructors,
       Feature.SubsetTypeTests,
       Feature.AllUnderscoreExternalModuleNames,
-      Feature.RuntimeCoverageReport
+      Feature.RuntimeCoverageReport,
+      Feature.StandardLibrariesActionsExterns
     };
 
     public override string ModuleSeparator => "_";
